Lott/Data/String.lean
@@ -1,0 +1,69 @@
+import Lott.Data.Substring
+
+namespace String
+
+private
+def toPascalParts (s : String) : Array String := Id.run do
+  let rawParts := s.data.splitBy (·.isUpper == ·.isUpper)
+  let mut parts : Array String := #[]
+  for rawPart in rawParts do
+    if rawPart[0]!.isLower then
+      if let some last := parts.back? then
+        parts := parts.pop.push <| last ++ ⟨rawPart⟩
+      else
+        parts := parts.push ⟨rawPart⟩
+      continue
+
+    if rawPart.length > 1 then
+      parts := parts ++ #[⟨rawPart.dropLast⟩, rawPart.getLast!.toString]
+    else
+      parts := parts.push ⟨rawPart⟩
+  return parts
+
+def pascalToSnake (s : String) : String :=
+  "_".intercalate <| s.toPascalParts.toList.map String.toLower
+
+def pascalToTitle (s : String) : String := " ".intercalate s.toPascalParts.toList
+
+def texEscape (s : String) : String :=
+  join <| s.data.map fun
+    | c@'&' | c@'%' | c@'$' | c@'#' | c@'_' | c@'{' | c@'}' => "\\" ++ c.toString
+    | '~' => "\\textasciitilde"
+    | '^' => "\\textasciicircum"
+    | '\\' => "\\textbackslash"
+    | c => c.toString
+
+/-
+Based on `munge` in libcpp/mkdeps.cc from the GCC source code. This is
+imperfect as some special characters can't be escaped.
+-/
+def makeEscape (s : String) : String := Id.run do
+  let mut res := ""
+  let mut slashes := 0
+  for c in s.data do
+    match c with
+    | '\\' => slashes := slashes + 1
+    | '$' =>
+      res := res.push '$'
+      slashes := 0
+    | ':' =>
+      res := res.push '\\'
+      slashes := 0
+    | ' ' | '\t' =>
+      /-
+      `munge`'s source contains a comment here that says: "A
+      space or tab preceded by 2N+1 backslashes represents N
+      backslashes followed by space..."
+      -/
+      res := res.pushn '\\' <| slashes + 1
+      slashes := 0
+    | '#' =>
+      res := res.push '\\'
+      slashes := 0
+    | _ => slashes := 0
+    res := res.push c
+  res
+
+def dropPrefixes (s pre : String) : Substring := s.toSubstring.dropPrefixes pre.toSubstring
+
+end String
