Lott/Elab/NoTexJudgement.lean
@@ -1,0 +1,13 @@
+import Lott.Parser.NoTexJudgement
+
+namespace Lott
+
+open Lean
+
+@[macro Lott.judgementEmbed]
+private
+def noTexJudgementImpl : Macro := fun stx => do
+  let `([[$j:Lott.Judgement notex]]) := stx | Macro.throwUnsupported
+  ``([[$j:Lott.Judgement]])
+
+end Lott
