Lott/Linter/UnusedVariables.lean
@@ -1,0 +1,32 @@
+import Lean.Linter
+
+namespace Lean.Linter
+
+/- Term embedding syntax. -/
+
+/-
+You can't put a hole inside an embedding to ignore something, so it's generally desirable to not be
+bugged about embedding pattern variables being unused.
+-/
+register_option linter.unusedVariables.lottSymbolEmbeddingPatternVars : Bool := {
+  defValue := false
+  descr :=
+    "enable the 'unused variables' linter to mark unused lott symbol embedding pattern variables"
+}
+
+def getLinterUnusedVariablesLottSymbolEmbeddingPatternVars (o : Options) : Bool :=
+  o.get linter.unusedVariables.lottSymbolEmbeddingPatternVars.name
+    (Lean.Linter.getLinterUnusedVariables o &&
+      linter.unusedVariables.lottSymbolEmbeddingPatternVars.defValue)
+
+@[unused_variables_ignore_fn]
+private
+def symbolEmbeddingPatternVars : Lean.Linter.IgnoreFunction := fun _ stack opts =>
+  !getLinterUnusedVariablesLottSymbolEmbeddingPatternVars opts && (
+    let stackBeforeMatchAlt := stack.takeWhile fun (stx, _) =>
+      !stx.isOfKind ``Lean.Parser.Term.matchAlt
+    stackBeforeMatchAlt.length != stack.length &&
+      stackBeforeMatchAlt.any fun (stx, _) => stx.isOfKind `Lott.symbolEmbed
+  )
+
+end Lean.Linter
