Lott/Parser/NoTexJudgement.lean
@@ -1,0 +1,7 @@
+import Lott.Parser
+
+namespace Lott
+
+syntax (name := noTexJudgement) Lott.Judgement " notex" : Lott.Judgement
+
+end Lott
