LottExamples/Lambda.lean
@@ -9,25 +9,27 @@ nonterminal Term, e :=
   | x             : var
   | "λ " x ". " e : lam (bind x in e)
   | e₀ e₁         : app
-  | "(" e ")"     : paren (expand := return e)
+  | "(" e ")"     : paren notex (expand := return e)
 
 -- Alpha reduction is not included since locally nameless representation makes it meaningless.
 
-judgement_syntax e " ->ᵦ " e' : BetaReduction
+judgement_syntax e " ->ᵦ " e' : BetaReduction (tex := s!"{e} \\; \\lottsym\{\\stackrel\{β}\{→}} \\; {e'}")
 
 judgement BetaReduction :=
 
-─────────────────────── mk
-(λ x. e₀) e₁ ->ᵦ e₀^^e₁
+───────────────────────── mk
+(λ x. e₀) e₁ ->ᵦ e₀^^e₁/x
 
 judgement_syntax "lc" "(" e ")" : Term.VarLocallyClosed
 
-judgement_syntax e " ->η " e' : EtaReduction
+judgement_syntax e " ->η " e' : EtaReduction (tex := s!"{e} \\; \\lottsym\{\\stackrel\{η}\{→}} \\; {e'}")
 
 judgement EtaReduction :=
 
 lc(e)
 ──────────────── mk
 λ x. e x$0 ->η e
+
+#filter "Lambda/intro.tex.lotttmpl"
 
 end LottExamples.Lambda
