lakefile.lean
@@ -1,10 +1,15 @@
 import Lake
 open Lake DSL
 
-package lott
+-- TODO: Use lib leanOptions for everything instead of args once string escaping is fixed.
+
+package lott where
+  moreGlobalServerArgs := #[s!"-Dweak.lott.tex.output.dir={__dir__}"]
 
 require aesop from git "https://github.com/leanprover-community/aesop" @ "v4.17.0"
 
 lean_lib Lott
 
-lean_lib LottExamples
+lean_lib LottExamples where
+  leanOptions := #[⟨`lott.tex.output.sourceRelative, false⟩]
+  moreLeanArgs := #[s!"-Dlott.tex.output.dir={__dir__}"]
